pr/274/head/lf/terse/lean/LF/Basics.lean
@@ -2,6 +2,8 @@ import LF.SFLCompat
 
 -- # Basics: Functional Programming in Lean
 
+set_option pp.fieldNotation false
+
 -- ## Data and Functions
 
 -- In Lean, we can build practically everything from first
